\documentclass[a4paper,16pt]{jsarticle}

% 余白の設定
\setlength{\textwidth}{\fullwidth}
\setlength{\textheight}{40\baselineskip}
\addtolength{\textheight}{\topskip}
\setlength{\voffset}{-0.2in}
\setlength{\topmargin}{0pt}
\setlength{\headheight}{0pt}
\setlength{\headsep}{0pt}

% パッケージ
\usepackage[dvipdfmx]{hyperref,graphicx}		% 画像
\hypersetup{
	colorlinks=true, % リンクに色をつけない設定
	bookmarks=true, % 以下ブックマークに関する設定
	bookmarksnumbered=true,
	pdfborder={0 0 0},
	bookmarkstype=toc
}
\usepackage{amsmath, amssymb}		% ギリシャ文字
\usepackage{bm}				% 数式　\bm{a} aベクトル
\usepackage{comment}			% コメント
\usepackage{siunitx}			% SI単位
\usepackage{framed}			% 枠組み
\usepackage{braket}     % ブラケット記法

\newtheorem{theorem}{定理}
\newtheorem{proof}{証明}
\newcommand{\qed}{\qquad $\blacksquare$}

\begin{comment}
　複数行に渡るコメントの書き方
　\usepackage{comment}が必要。
\end{comment}

% section前に改ページ
\makeatletter
\def\section{\newpage\@startsection {section}{1}{\z@}{-3.5ex plus -1ex minus -.2ex}{2.3 ex plus .2ex}{\Large\bf}}
\makeatother

% 数式番号をいい感じに
\makeatletter
% \renewcommand{\theequation}{\arabic{chapter}-\arabic{section}-\arabic{equation}}
	\renewcommand{\theequation}{\arabic{section}-\arabic{equation}}
  \@addtoreset{equation}{section}
\makeatother

\title{Ex09}
\author{ゆきちゃん}
\date{\today}

\begin{document}
\maketitle

\begin{itemize}
	\item Given a causal discrete-time LT$1$ system $y[n]-\frac{3}{4}y[n-1]+\frac{1}{8}y[n-2] = x[n]$, where $x[n]$ and $y[n]$ are the input and output of the system, respectively.
\end{itemize}
\begin{enumerate}
	\item Determine the transfer function $H(z)$
	\item Find its impulse response $h[n]$
	\item Fint its step response $s[n]$
\end{enumerate}

Answer:

\begin{enumerate}
	\item Taking the z-transform of the system equation, we have
	\begin{equation}
		Y(z) - \dfrac{3}{4}z^{-1}Y(z) + \dfrac{1}{8}z^{-2}Y(z) = X(z)
	\end{equation}
	Thus,
	\begin{equation}
		H(z) = \dfrac{Y(z)}{X(z)} = \dfrac{z^2}{(z-\frac{1}{2})(z-\frac{1}{4})}
	\end{equation}

	\item Using partial-fraction expansion, we have
	\begin{equation}
		\dfrac{H(z)}{z} = \dfrac{z}{(z-\frac{1}{2})(z-\frac{1}{4})} = \dfrac{c_1}{z-\frac{1}{2}} + \dfrac{c_2}{z-\frac{1}{4}}
	\end{equation}
	where, $c_1 = 2$,$c_2 = -1$

	Thus,
	\begin{equation}
		H(z) = \dfrac{2z}{z-\frac{1}{2}} - \dfrac{z}{z-\frac{1}{4}} = \dfrac{2}{1-\frac{1}{2}z^{-1}} - \dfrac{1}{1-\frac{1}{4}z^{-1}}
	\end{equation}
	Taking the inverse z-transform
	\footnote{$z[a^nu[n]] = \dfrac{1}{1-az^{-1}},~(|z| > |a|)$}
	of $H(z)$, we get
	\begin{equation}
		h(n) = 2\left(\dfrac{1}{2}\right)^n u[n] - \left(\dfrac{1}{4}\right)^n u[n]
	\end{equation}

	\item From the table in slide P19, we have the z-transform pair for step signal $x[n] = u[n] \overset{zT}{\iff} X(z) = \dfrac{z}{z-1}$
	Thus, the steo response
	\begin{equation}
		Y(z) = H(z)X(z) = \dfrac{2z^2}{(z-\frac{1}{2})(z-1)} - \dfrac{z^2}{(z-\frac{1}{4})(z-1)}
	\end{equation}
	Using partial-fraction expansion, we have
	\begin{align}
		\dfrac{Y(z)}{z} &= \dfrac{2z}{(z-\frac{1}{2})(z-1)} - \dfrac{z}{(z-\frac{1}{4})(z-1)} \\
		&= \dfrac{c_1}{z-\frac{1}{2}} + \dfrac{c_2}{z-1} + \dfrac{c_3}{z-\frac{1}{4}}
	\end{align}
	where, $c_1 = -2, c_2 = \dfrac{8}{3}, c_3 = \dfrac{1}{3}$

	Thus,
	\begin{equation}
		Y(z) = 	\dfrac{-2z}{z-\frac{1}{2}} + \dfrac{8z}{(3(z-1)} + \dfrac{z}{3(z-\frac{1}{4})}
	\end{equation}
	Taking the inverse z-transform of $Y(z)$, we obtain the step response $s[n]$
	\begin{equation}
		s[n] = y[n] = -2\left(\dfrac{1}{2}\right)^n u[n] + \dfrac{8}{3}u[n] + \dfrac{1}{3} \left(\dfrac{1}{4}\right)^n u[n]
	\end{equation}
\end{enumerate}


\end{document}
