\documentclass[a4paper,16pt]{jsarticle}

% 余白の設定
\setlength{\textwidth}{\fullwidth}
\setlength{\textheight}{40\baselineskip}
\addtolength{\textheight}{\topskip}
\setlength{\voffset}{-0.2in}
\setlength{\topmargin}{0pt}
\setlength{\headheight}{0pt}
\setlength{\headsep}{0pt}

% パッケージ
\usepackage[dvipdfmx]{hyperref,graphicx}		% 画像
\hypersetup{
	colorlinks=true, % リンクに色をつけない設定
	bookmarks=true, % 以下ブックマークに関する設定
	bookmarksnumbered=true,
	pdfborder={0 0 0},
	bookmarkstype=toc
}
\usepackage{amsmath, amssymb}		% ギリシャ文字
\usepackage{bm}				% 数式　\bm{a} aベクトル
\usepackage{comment}			% コメント
\usepackage{siunitx}			% SI単位
\usepackage{framed}			% 枠組み
\usepackage{braket}     % ブラケット記法

\newtheorem{theorem}{定理}
\newtheorem{proof}{証明}
\newcommand{\qed}{\qquad $\blacksquare$}

\begin{comment}
　複数行に渡るコメントの書き方
　\usepackage{comment}が必要。
\end{comment}

% section前に改ページ
\makeatletter
\def\section{\newpage\@startsection {section}{1}{\z@}{-3.5ex plus -1ex minus -.2ex}{2.3 ex plus .2ex}{\Large\bf}}
\makeatother

% 数式番号をいい感じに
\makeatletter
% \renewcommand{\theequation}{\arabic{chapter}-\arabic{section}-\arabic{equation}}
	\renewcommand{\theequation}{\arabic{section}-\arabic{equation}}
  \@addtoreset{equation}{section}
\makeatother

\title{Ex10}
\author{ゆきちゃん}
\date{\today}

\begin{document}
\maketitle

\begin{itemize}
	\item Given a unit sample response of an FIR filter si
	\begin{equation}
		h[n] =
		\begin{cases}
			\alpha^n, & 0 \leq n \leq 6 \\
			0,        & otherwise
		\end{cases}
	\end{equation}
\end{itemize}

\begin{enumerate}
	\item Draw the direct form implementation of this filter
	\item Show that the corresponding transfer function is
	\begin{equation}
		H(z) = \dfrac{1 - \alpha^7 z{-7}}{1 - \alpha z^{-1}}
	\end{equation}
\end{enumerate}

Answer:

\begin{enumerate}
	\item 略
	\item The transfer function is,
	\begin{align}
		H(z) &= \sum_{n=-\infty}^\infty h[n]z^{-n} \\
		&= \sum_{n=0}^{6} \alpha^n z^{-n} \\
		&= 1 + \sum_{n=1}^{6} \alpha^n z^{-n} \\
		&= 1 + \sum_{n=1}^{6} \dfrac{\alpha}{z}\left(\dfrac{\alpha}{z}\right)^{n-1} \\
		&= 1 + \dfrac{\frac{\alpha}{z}(1-(\frac{\alpha}{z})^6)}{1-\frac{\alpha}{z}} \\
		&= \dfrac{1-\alpha^7 z^{-7}}{1-\alpha z^{-1}}
	\end{align}
\end{enumerate}

\end{document}
